Verify new HigherOrderExample (#434)
Pretty straightforward use of simple plus future.

Simple doesn't allow closing (it would require some permission tokens to
avoid send after close and double close), so the code doesn't actually
clean up the workers by closing.

Depends on https://github.com/goose-lang/goose/pull/154

new/code/github_com/goose_lang/goose/testdata/examples/channel.v
@@ -8,6 +8,8 @@ Definition chan_spec_raw_examples : go_string := "github.com/goose-lang/goose/te
 
 Module chan_spec_raw_examples.
 
+Module request. Definition id : go_string := "github.com/goose-lang/goose/testdata/examples/channel.request"%go. End request.
+
 Section code.
 Context `{ffi_syntax}.
 
@@ -530,6 +532,90 @@ Definition LeakyBufferPipelineⁱᵐᵖˡ : val :=
     else do:  #());;;
     return: #()).
 
+Definition request : go_type := structT [
+  "f" :: funcT;
+  "result" :: chanT stringT
+].
+#[global] Typeclasses Opaque request.
+#[global] Opaque request.
+
+Definition mkRequest : go_string := "github.com/goose-lang/goose/testdata/examples/channel.mkRequest"%go.
+
+(* go: higher_order.go:8:6 *)
+Definition mkRequestⁱᵐᵖˡ : val :=
+  λ: "f",
+    exception_do (let: "f" := (mem.alloc "f") in
+    return: (let: "$f" := (![#funcT] "f") in
+     let: "$result" := (chan.make #stringT #(W64 1)) in
+     struct.make #request [{
+       "f" ::= "$f";
+       "result" ::= "$result"
+     }])).
+
+Definition ho_worker : go_string := "github.com/goose-lang/goose/testdata/examples/channel.ho_worker"%go.
+
+(* go: higher_order.go:12:6 *)
+Definition ho_workerⁱᵐᵖˡ : val :=
+  λ: "c",
+    exception_do (let: "c" := (mem.alloc "c") in
+    let: "$range" := (![type.chanT #request] "c") in
+    (let: "r" := (mem.alloc (type.zero_val #request)) in
+    chan.for_range #request "$range" (λ: "$key",
+      do:  ("r" <-[#request] "$key");;;
+      do:  (let: "$chan" := (![type.chanT #stringT] (struct.field_ref #request #"result"%go "r")) in
+      let: "$v" := ((![#funcT] (struct.field_ref #request #"f"%go "r")) #()) in
+      chan.send #stringT "$chan" "$v")));;;
+    return: #()).
+
+Definition HigherOrderExample : go_string := "github.com/goose-lang/goose/testdata/examples/channel.HigherOrderExample"%go.
+
+(* go: higher_order.go:18:6 *)
+Definition HigherOrderExampleⁱᵐᵖˡ : val :=
+  λ: <>,
+    exception_do (let: "c" := (mem.alloc (type.zero_val (type.chanT #request))) in
+    let: "$r0" := (chan.make #request #(W64 0)) in
+    do:  ("c" <-[type.chanT #request] "$r0");;;
+    let: "$a0" := (![type.chanT #request] "c") in
+    let: "$go" := (func_call #ho_worker) in
+    do:  (Fork ("$go" "$a0"));;;
+    let: "$a0" := (![type.chanT #request] "c") in
+    let: "$go" := (func_call #ho_worker) in
+    do:  (Fork ("$go" "$a0"));;;
+    let: "r1" := (mem.alloc (type.zero_val #request)) in
+    let: "$r0" := (let: "$a0" := (λ: <>,
+      exception_do (return: (#("hello"%go ++ " world"%go)))
+      ) in
+    (func_call #mkRequest) "$a0") in
+    do:  ("r1" <-[#request] "$r0");;;
+    let: "r2" := (mem.alloc (type.zero_val #request)) in
+    let: "$r0" := (let: "$a0" := (λ: <>,
+      exception_do (return: (#"HELLO"%go))
+      ) in
+    (func_call #mkRequest) "$a0") in
+    do:  ("r2" <-[#request] "$r0");;;
+    let: "r3" := (mem.alloc (type.zero_val #request)) in
+    let: "$r0" := (let: "$a0" := (λ: <>,
+      exception_do (return: (#(("w"%go ++ "o"%go) ++ "rld"%go)))
+      ) in
+    (func_call #mkRequest) "$a0") in
+    do:  ("r3" <-[#request] "$r0");;;
+    do:  (let: "$chan" := (![type.chanT #request] "c") in
+    let: "$v" := (![#request] "r1") in
+    chan.send #request "$chan" "$v");;;
+    do:  (let: "$chan" := (![type.chanT #request] "c") in
+    let: "$v" := (![#request] "r2") in
+    chan.send #request "$chan" "$v");;;
+    do:  (let: "$chan" := (![type.chanT #request] "c") in
+    let: "$v" := (![#request] "r3") in
+    chan.send #request "$chan" "$v");;;
+    let: "responses" := (mem.alloc (type.zero_val #sliceT)) in
+    let: "$r0" := ((let: "$sl0" := (Fst (chan.receive #stringT (![type.chanT #stringT] (struct.field_ref #request #"result"%go "r1")))) in
+    let: "$sl1" := (Fst (chan.receive #stringT (![type.chanT #stringT] (struct.field_ref #request #"result"%go "r2")))) in
+    let: "$sl2" := (Fst (chan.receive #stringT (![type.chanT #stringT] (struct.field_ref #request #"result"%go "r3")))) in
+    slice.literal #stringT ["$sl0"; "$sl1"; "$sl2"])) in
+    do:  ("responses" <-[#sliceT] "$r0");;;
+    return: (![#sliceT] "responses")).
+
 Definition worker : go_string := "github.com/goose-lang/goose/testdata/examples/channel.worker"%go.
 
 (* go: parallel_search_replace.go:13:6 *)
@@ -627,9 +713,9 @@ Definition SearchReplaceⁱᵐᵖˡ : val :=
 
 Definition vars' : list (go_string * go_type) := [].
 
-Definition functions' : list (go_string * val) := [(sys_hello_world, sys_hello_worldⁱᵐᵖˡ); (HelloWorldAsync, HelloWorldAsyncⁱᵐᵖˡ); (HelloWorldSync, HelloWorldSyncⁱᵐᵖˡ); (HelloWorldCancellable, HelloWorldCancellableⁱᵐᵖˡ); (HelloWorldWithTimeout, HelloWorldWithTimeoutⁱᵐᵖˡ); (DSPExample, DSPExampleⁱᵐᵖˡ); (fibonacci, fibonacciⁱᵐᵖˡ); (fib_consumer, fib_consumerⁱᵐᵖˡ); (select_nb_no_panic, select_nb_no_panicⁱᵐᵖˡ); (select_ready_case_no_panic, select_ready_case_no_panicⁱᵐᵖˡ); (TestHelloWorldSync, TestHelloWorldSyncⁱᵐᵖˡ); (TestHelloWorldWithTimeout, TestHelloWorldWithTimeoutⁱᵐᵖˡ); (TestDSPExample, TestDSPExampleⁱᵐᵖˡ); (TestFibConsumer, TestFibConsumerⁱᵐᵖˡ); (TestSelectNbNoPanic, TestSelectNbNoPanicⁱᵐᵖˡ); (TestSelectReadyCaseNoPanic, TestSelectReadyCaseNoPanicⁱᵐᵖˡ); (load, loadⁱᵐᵖˡ); (process, processⁱᵐᵖˡ); (client, clientⁱᵐᵖˡ); (server, serverⁱᵐᵖˡ); (LeakyBufferPipeline, LeakyBufferPipelineⁱᵐᵖˡ); (worker, workerⁱᵐᵖˡ); (SearchReplace, SearchReplaceⁱᵐᵖˡ)].
+Definition functions' : list (go_string * val) := [(sys_hello_world, sys_hello_worldⁱᵐᵖˡ); (HelloWorldAsync, HelloWorldAsyncⁱᵐᵖˡ); (HelloWorldSync, HelloWorldSyncⁱᵐᵖˡ); (HelloWorldCancellable, HelloWorldCancellableⁱᵐᵖˡ); (HelloWorldWithTimeout, HelloWorldWithTimeoutⁱᵐᵖˡ); (DSPExample, DSPExampleⁱᵐᵖˡ); (fibonacci, fibonacciⁱᵐᵖˡ); (fib_consumer, fib_consumerⁱᵐᵖˡ); (select_nb_no_panic, select_nb_no_panicⁱᵐᵖˡ); (select_ready_case_no_panic, select_ready_case_no_panicⁱᵐᵖˡ); (TestHelloWorldSync, TestHelloWorldSyncⁱᵐᵖˡ); (TestHelloWorldWithTimeout, TestHelloWorldWithTimeoutⁱᵐᵖˡ); (TestDSPExample, TestDSPExampleⁱᵐᵖˡ); (TestFibConsumer, TestFibConsumerⁱᵐᵖˡ); (TestSelectNbNoPanic, TestSelectNbNoPanicⁱᵐᵖˡ); (TestSelectReadyCaseNoPanic, TestSelectReadyCaseNoPanicⁱᵐᵖˡ); (load, loadⁱᵐᵖˡ); (process, processⁱᵐᵖˡ); (client, clientⁱᵐᵖˡ); (server, serverⁱᵐᵖˡ); (LeakyBufferPipeline, LeakyBufferPipelineⁱᵐᵖˡ); (mkRequest, mkRequestⁱᵐᵖˡ); (ho_worker, ho_workerⁱᵐᵖˡ); (HigherOrderExample, HigherOrderExampleⁱᵐᵖˡ); (worker, workerⁱᵐᵖˡ); (SearchReplace, SearchReplaceⁱᵐᵖˡ)].
 
-Definition msets' : list (go_string * (list (go_string * val))) := [].
+Definition msets' : list (go_string * (list (go_string * val))) := [(request.id, []); (ptrT.id request.id, [])].
 
 #[global] Instance info' : PkgInfo channel.chan_spec_raw_examples :=
   {|
